\begin{document}
$
(1) \hspace{10mm} P (x) = a_{n}x^{n} + a_{n-1}x^{n-1} + ... + a_{1}x + a_{0} \hspace{10 mm} (a_{n} \neq 0) \\
\vspace{5mm} x \in R \\
\vspace{5mm} z_{1}, \ldots, z_{n} \\
\vspace{5mm} (2) \hspace{10mm} P(x) = a_{n}(x - z_{1})(x - z_{2})\dots(x - z_{n}) \\
\vspace{5mm} P(z_{i}) = 0 \\
\vspace{5mm} (x - z)^{r} \\
\vspace{5mm} P(z) = 0 \\
\vspace{5mm} P(\bar{z}) = 0 \\
\vspace{5mm} (s \geq 1)  \\
\vspace{5mm} ((x - z)(x - \bar{z}))^{s} \\
\vspace{5mm} z = \alpha + i\beta \\
\vspace{5mm} \bar{z} = \alpha - i\beta \\
\vspace{5mm} ((x - z)(x - \bar{z}))^{s} = (x^{2} - 2\alpha x + (\alpha^{2} + \beta^{2})^{s} = (x^{2} + px + q)^{s} \\
\vspace{5mm} p = -2\alpha \\
\vspace{5mm} q = \alpha^{2} + \beta^{2} \\
\vspace{5mm} p^{2} - 4q < 0 \\
\vspace{5mm} P(x) = a_{n}(x - x_{1})^{r_{1}}(x - x_{2})^{r_{2}}\dots(x - x_{k})^{r_{2}}(x^{2} + p_{1}x + q_{1})^{s_{1}}\dots(x^{2} + p_{m}x + q_{m})^{s_{m}} \\
\vspace{5mm} a_{0}, a_{1}, \ldots, a_{n} \\
\vspace{5mm} x_{1}, \ldots, x_{k} \\
\vspace{5mm} r_{1}, \ldots, r_{k} \\
\vspace{2mm}
$

\end{document}
